(1) The address of the adversary is now fixed at [1], and in UCBasicTypes.ec, adv is an alias for this. Consequently, envport now takes only two arguments in its real form: the address of the functionality, and the port in question. It still has the same meaning as before, except that the adversary's address is fixed. (In the UC DSL, as before, it just takes in a port.) Consequently, two lemmas about envport that didn't work as rewriting hints now do, and are included in the default rewriting database. This means that the .uci script for the SMC2 example now runs with no usage of SMT at all. (And a prover directive enforces this.)
(2) Some redundant uses of simplification in the interpreter have been
removed.  (Thanks to Galois for suggesting this.)

uc-dsl/ucdsl-proj/src/ucInterpreter.ml
@@ -227,8 +227,10 @@ let env_root_addr_form : form = form_of_expr mhr env_root_addr_op
 
 let env_root_port_form : form = form_of_expr mhr env_root_port_op
 
-let envport_form (func : form) (adv : form) (pt : form) : form =
-  f_app (form_of_expr mhr envport_op) [func; adv; pt] tbool
+let adv_addr_form : form = form_of_expr mhr adv_addr_op
+
+let envport_form (func : form) (pt : form) : form =
+  f_app (form_of_expr mhr envport_op) [func; pt] tbool
 
 let inc_form (addr1 : form) (addr2 : form) : form =
   f_app (form_of_expr mhr inc_op) [addr1; addr2] tbool
@@ -286,21 +288,18 @@ let support_form (ty : ty) (d : form) (x : form) : form =
 type global_context = LDecl.hyps
 
 let func_id         : EcIdent.t = EcIdent.create "func"
-let adv_id          : EcIdent.t = EcIdent.create "adv"
 let inc_func_adv_id : EcIdent.t = EcIdent.create "IncFuncAdv"
 
 let func_form : form = f_local func_id addr_ty
-let adv_form  : form = f_local adv_id addr_ty
 
 let gc_create (env : env) : global_context =
   let locs =
     [
       (func_id, EcBaseLogic.LD_var (addr_ty, None));
-      (adv_id,  EcBaseLogic.LD_var (addr_ty, None));
       (inc_func_adv_id,
        EcBaseLogic.LD_hyp
        (form_of_expr mhr
-        (e_app inc_op [e_local func_id addr_ty; e_local adv_id addr_ty]
+        (e_app inc_op [e_local func_id addr_ty; adv_addr_op]
          tbool)))
     ] in
   LDecl.init env ~locals:(List.rev locs) []
@@ -584,25 +583,23 @@ type local_context_base =
   | LCB_Bound   of EcIdent.t * form  (* bound identifier - state param or
                                         of message match clause *)
   | LCB_Var     of EcIdent.t * ty    (* local variable *)
-  | LCB_EnvPort of form * form       (* both of type address *)
+  | LCB_EnvPort of form
   | LCB_IntPort of EcIdent.t * form  (* of type port *)
 
 let lc_create (gc : global_context) (dbs : rewriting_dbs)
     (lcbs : local_context_base list) : local_context =
-  let simpl = simplify_formula gc dbs in
   [EcIdent.Mid.of_list
    (List.map
     (fun lcb ->
        match lcb with
-       | LCB_Bound (id, form)    -> (id, simpl form)
-       | LCB_Var (id, ty)        ->
+       | LCB_Bound (id, form) -> (id, form)
+       | LCB_Var (id, ty)     ->
            (id, f_op EcCoreLib.CI_Witness.p_witness [ty] ty)
-       | LCB_EnvPort (func, adv) ->
+       | LCB_EnvPort func     ->
            (envport_id,
-            simpl
             (f_app (form_of_expr mhr envport_op)
-             [func; adv] (tfun port_ty tbool)))
-       | LCB_IntPort (id, port)  -> (id, simpl port))
+             [func] (tfun port_ty tbool)))
+       | LCB_IntPort (id, port)  -> (id, port))
     lcbs)]
 
 let lc_find_key_from_sym (map : 'a EcIdent.Mid.t) (sym : symbol)
@@ -617,12 +614,11 @@ let lc_find_key_from_sym (map : 'a EcIdent.Mid.t) (sym : symbol)
 
 let lc_update_var (gc : global_context) (lc : local_context)
     (dbs : rewriting_dbs) (id : symbol) (f : form) : local_context =
-  let f = simplify_formula gc dbs f in
   let (lc_base, lc_rest) = (List.hd lc, List.tl lc) in
   let id = Option.get (lc_find_key_from_sym lc_base id) in
   EcIdent.Mid.change (fun _ -> Some f) id lc_base :: lc_rest
 
-let lc_apply (gc : global_context) (lc : local_context)
+let lc_apply (simpl : bool) (gc : global_context) (lc : local_context)
     (dbs : rewriting_dbs) (e : expr) : form =
   let f = form_of_expr mhr e in
   let map =
@@ -635,7 +631,7 @@ let lc_apply (gc : global_context) (lc : local_context)
     (fun acc (x, f) -> Fsubst.f_bind_local acc x f)
     Fsubst.f_subst_id (EcIdent.Mid.bindings map) in
   let f = Fsubst.f_subst subst f in
-  simplify_formula gc dbs f
+  if simpl then simplify_formula gc dbs f else f
 
 let push (lc : local_context) (fr : local_context_frame) : local_context =
   lc @ [fr]
@@ -1660,7 +1656,7 @@ exception StepBlockedPortOrAddrCompare
 let step_assign (gc : global_context) (lc : local_context)
     (pi : prover_infos) (dbs : rewriting_dbs)
     (lhs : lhs) (expr : expr) : local_context =
-  let form = lc_apply gc lc dbs expr in
+  let form = lc_apply true gc lc dbs expr in
   match lhs with
   | LHSSimp id   -> lc_update_var gc lc dbs (unloc id) form
   | LHSTuple ids ->
@@ -1679,7 +1675,7 @@ let step_sample (gc : global_context) (lc : local_context)
     (pi : prover_infos) (dbs : rewriting_dbs)
     (lhs : lhs) (expr : expr)
       : global_context * local_context * symbol =
-  let form = lc_apply gc lc dbs expr in
+  let form = lc_apply true gc lc dbs expr in
   let ty = Option.get (as_tdistr (EcEnv.Ty.hnorm form.f_ty (env_of_gc gc))) in
   match lhs with
   | LHSSimp id   ->
@@ -1705,7 +1701,7 @@ let step_if_then_else (gc : global_context) (lc : local_context)
     (pi : prover_infos) (dbs : rewriting_dbs)
     (expr : expr) (inss_then : instr_interp list)
     (inss_else_opt : instr_interp list option) : instr_interp list =
-  let expr_gc_form = lc_apply gc lc dbs expr in
+  let expr_gc_form = lc_apply false gc lc dbs expr in
   if try eval_bool_form_to_bool gc pi dbs expr_gc_form with
      | ECProofEngine -> raise StepBlockedIf
   then inss_then
@@ -1715,7 +1711,7 @@ let step_match (gc : global_context) (lc : local_context)
     (pi : prover_infos) (dbs : rewriting_dbs)
     (expr : expr) (clauses : match_clause_interp list)
       : local_context * instr_interp list =
-  let form = lc_apply gc lc dbs expr in
+  let form = lc_apply false gc lc dbs expr in
   let (form_constr, form_args) =
     try deconstruct_datatype_value gc pi dbs form with
     | ECProofEngine -> raise StepBlockedMatch in
@@ -1761,7 +1757,7 @@ let rw_step_send_and_transition_from_ideal_fun (c : config_real_running)
          path           = path;
          args           = msg_args;
          dest_port_form =
-           make_port_form adv_form (int_form base)} in
+           make_port_form adv_addr_form (int_form base)} in
       let () = check_sme_port_index_consistency c.maps c.gc pi dbs sme in
       (ConfigRealSending
        {maps = c.maps;
@@ -1783,7 +1779,7 @@ let rw_step_send_and_transition_from_ideal_fun (c : config_real_running)
       let path = {inter_id_path = root :: iip; msg = msg} in
       if try eval_bool_form_to_bool c.gc pi dbs
              (envport_form (addr_concat_form func_form (addr_make_form rel))
-              adv_form port_form) with
+              port_form) with
          | ECProofEngine -> raise StepBlockedPortOrAddrCompare
       then let sme =
              SMET_Ord
@@ -1888,7 +1884,7 @@ let rw_step_send_and_transition_from_real_fun_party_to_env_or_adv
          path           = path;
          args           = msg_args;
          dest_port_form =
-           make_port_form adv_form (int_form adv_pi)} in
+           make_port_form adv_addr_form (int_form adv_pi)} in
       let () = check_sme_port_index_consistency c.maps c.gc pi dbs sme in
       (ConfigRealSending
        {maps = c.maps;
@@ -1906,7 +1902,7 @@ let rw_step_send_and_transition_from_real_fun_party_to_env_or_adv
       let path = {inter_id_path = root :: iip; msg = msg} in
       if try eval_bool_form_to_bool c.gc pi dbs
              (envport_form (addr_concat_form func_form (addr_make_form rel))
-              adv_form port_form) with
+              port_form) with
          | ECProofEngine -> raise StepBlockedPortOrAddrCompare
       then let sme =
              SMET_Ord
@@ -1968,16 +1964,16 @@ let rw_step_send_and_transition (c : config_real_running) (pi : prover_infos)
   let {path; args = msg_args; port_expr} = msg_expr in
   let {inter_id_path = iip; msg} = unloc path in
   let msg_args =
-    List.map (fun arg -> lc_apply c.gc c.lc dbs arg) (unloc msg_args) in
+    List.map (fun arg -> lc_apply true c.gc c.lc dbs arg) (unloc msg_args) in
   let port_form =
     match port_expr with
     | None      -> None
-    | Some expr -> Some (lc_apply c.gc c.lc dbs expr) in
+    | Some expr -> Some (lc_apply true c.gc c.lc dbs expr) in
   let {UcTypedSpec.id = state_id; UcTypedSpec.args = state_args} =
     state_expr in
   let state_id = unloc state_id and state_args = unloc state_args in
   let state_args =
-    List.map (fun arg -> lc_apply c.gc c.lc dbs arg) state_args in
+    List.map (fun arg -> lc_apply true c.gc c.lc dbs arg) state_args in
   let new_state = {id = state_id; args = state_args} in
   let new_rws =
     match c.rwrc with
@@ -2060,7 +2056,7 @@ let iw_step_send_and_transition_from_ideal_fun (c : config_ideal_running)
          path           = path;
          args           = msg_args;
          dest_port_form =
-           make_port_form adv_form (int_form base)} in
+           make_port_form adv_addr_form (int_form base)} in
       let () = check_sme_port_index_consistency c.maps c.gc pi dbs sme in
       (ConfigIdealSending
        {maps = c.maps;
@@ -2081,7 +2077,7 @@ let iw_step_send_and_transition_from_ideal_fun (c : config_ideal_running)
       let source_pi = get_pi_of_sub_interface c.maps root comp sub in
       let path = {inter_id_path = root :: iip; msg = msg} in
       if try eval_bool_form_to_bool c.gc pi dbs
-             (envport_form func_form adv_form port_form) with
+             (envport_form func_form port_form) with
          | ECProofEngine -> raise StepBlockedPortOrAddrCompare
       then let sme =
              SMET_Ord
@@ -2129,7 +2125,7 @@ let iw_step_send_and_transition_from_sim_basic_adv_left
     SMET_Ord
     {mode           = Adv;
      dir            = In;
-     src_port_form  = make_port_form adv_form (int_form base);
+     src_port_form  = make_port_form adv_addr_form (int_form base);
      path           = path;
      args           = msg_args;
      dest_port_form = make_port_form sim_rf_addr (int_form 1)} in
@@ -2206,7 +2202,7 @@ let iw_step_send_and_transition_from_sim_comp_adv_right
           src_port_form  = make_port_form sim_rf_addr (int_form porti);
           path           = path;
           args           = msg_args;
-          dest_port_form = make_port_form adv_form (int_form adv_pi)} in
+          dest_port_form = make_port_form adv_addr_form (int_form adv_pi)} in
        let () = check_sme_port_index_consistency c.maps c.gc pi dbs sme in
        (ConfigIdealSending
         {maps = c.maps;
@@ -2240,7 +2236,7 @@ let iw_step_send_and_transition_from_sim_comp_adv_right
              (int_form 1));
           path           = path;
           args           = List.map simpl msg_args;
-          dest_port_form = make_port_form adv_form (int_form adv_pi)} in
+          dest_port_form = make_port_form adv_addr_form (int_form adv_pi)} in
        let () = check_sme_port_index_consistency c.maps c.gc pi dbs sme in
        (ConfigIdealSending
         {maps = c.maps;
@@ -2281,16 +2277,16 @@ let iw_step_send_and_transition (c : config_ideal_running) (pi : prover_infos)
   let {path; args = msg_args; port_expr} = msg_expr in
   let {inter_id_path = iip; msg} = unloc path in
   let msg_args =
-    List.map (fun arg -> lc_apply c.gc c.lc dbs arg) (unloc msg_args) in
+    List.map (fun arg -> lc_apply true c.gc c.lc dbs arg) (unloc msg_args) in
   let port_form =
     match port_expr with
     | None      -> None
-    | Some expr -> Some (lc_apply c.gc c.lc dbs expr) in
+    | Some expr -> Some (lc_apply true c.gc c.lc dbs expr) in
   let {UcTypedSpec.id = state_id; UcTypedSpec.args = state_args} =
     state_expr in
   let state_id = unloc state_id and state_args = unloc state_args in
   let state_args =
-    List.map (fun arg -> lc_apply c.gc c.lc dbs arg) state_args in
+    List.map (fun arg -> lc_apply true c.gc c.lc dbs arg) state_args in
   let new_state = {id = state_id; args = state_args} in
   let new_iws =
     match c.iwrc with
@@ -2406,7 +2402,7 @@ let match_ord_sme_in_state (gc : global_context) (dbs : rewriting_dbs)
   let mm_binds =
     List.map (fun ((id, _), f) -> (LCB_Bound (id, f))) mm_binds in
   let envport_maybe =
-    if is_sim then [] else [LCB_EnvPort (addr, adv_form)] in
+    if is_sim then [] else [LCB_EnvPort addr] in
   let internal_ports =
     List.mapi
     (fun i (_, id) -> LCB_IntPort (id, port_of_addr (i + 1)))
@@ -2596,7 +2592,7 @@ let step_real_sending_config (c : config_real_sending) (pi : prover_infos)
        eval_bool_form_to_bool c.gc pi dbs
        (f_and
         (f_eq dest_addr func_form)
-        (envport_form func_form adv_form source_port))
+        (envport_form func_form source_port))
       then let (func_sp, base, _) = c.rw in
            let (root, fid) = func_sp in
            let ft = IdPairMap.find func_sp c.maps.fun_map in
@@ -2619,14 +2615,14 @@ let step_real_sending_config (c : config_real_sending) (pi : prover_infos)
     else if mode = Adv &&
             eval_bool_form_to_bool c.gc pi dbs
             (f_and
-             (f_eq dest_addr adv_form)
+             (f_eq dest_addr adv_addr_form)
               (f_or
                (f_and
                 (f_eq dest_pi (int_form 0))
                 (f_eq source_port env_root_port_form))
                (f_and
                 (int_le_form (int_form c.ig) dest_pi)
-                (envport_form func_form adv_form source_port))))
+                (envport_form func_form source_port))))
       then msg_out_of_sending_config (ConfigRealSending c) CtrlAdv
     else fail_out_of_running_or_sending_config (ConfigRealSending c) in
 
@@ -2794,9 +2790,9 @@ let step_real_sending_config (c : config_real_sending) (pi : prover_infos)
     if mode = Dir ||
        eval_bool_form_to_bool c.gc pi dbs
        (f_or
-        (addr_le_form adv_form dest_addr)
+        (addr_le_form adv_addr_form dest_addr)
         (f_or
-         (f_not (f_eq adv_form source_addr))
+         (f_not (f_eq adv_addr_form source_addr))
          (int_lt_form source_pi (int_form 0))))
       then fail_out_of_running_or_sending_config (ConfigRealSending c)
     else if eval_bool_form_to_bool c.gc pi dbs
@@ -3112,7 +3108,7 @@ let step_ideal_sending_config (c : config_ideal_sending) (pi : prover_infos)
        eval_bool_form_to_bool c.gc pi dbs
        (f_and
         (f_eq dest_addr func_form)
-        (envport_form func_form adv_form source_port))
+        (envport_form func_form source_port))
       then let (func_sp, base) = c.iw.iw_ideal_func in
            let ft = unloc (IdPairMap.find func_sp c.maps.fun_map) in
            let ifbt = ideal_fun_body_tyd_of ft in
@@ -3120,7 +3116,7 @@ let step_ideal_sending_config (c : config_ideal_sending) (pi : prover_infos)
     else if mode = Adv &&
             eval_bool_form_to_bool c.gc pi dbs
             (f_and
-             (f_eq dest_addr adv_form)
+             (f_eq dest_addr adv_addr_form)
               (f_or
                (f_and
                 (f_eq dest_pi (int_form 0))
@@ -3129,7 +3125,7 @@ let step_ideal_sending_config (c : config_ideal_sending) (pi : prover_infos)
                 (int_lt_form (int_form 0) dest_pi)
                 (f_and
                  (int_le_form (int_form c.ig) dest_pi)
-                 (envport_form func_form adv_form source_port)))))
+                 (envport_form func_form source_port)))))
       then msg_out_of_sending_config (ConfigIdealSending c) CtrlAdv
     else fail_out_of_running_or_sending_config (ConfigIdealSending c) in
 
@@ -3509,7 +3505,7 @@ let step_ideal_sending_config (c : config_ideal_sending) (pi : prover_infos)
 
   let from_sim_left_or_right (i : int) : config * effect =
     if eval_bool_form_to_bool c.gc pi dbs
-       (f_eq dest_addr adv_form)
+       (f_eq dest_addr adv_addr_form)
       then if i = List.length c.iws.other_sims_states - 1
            then msg_out_of_sending_config (ConfigIdealSending c) CtrlAdv
            else match find_sim_from_left (i + 1) with
@@ -3542,9 +3538,9 @@ let step_ideal_sending_config (c : config_ideal_sending) (pi : prover_infos)
     if mode = Dir ||
        eval_bool_form_to_bool c.gc pi dbs
        (f_or
-        (addr_le_form adv_form dest_addr)
+        (addr_le_form adv_addr_form dest_addr)
         (f_or
-         (f_not (f_eq adv_form source_addr))
+         (f_not (f_eq adv_addr_form source_addr))
          (int_lt_form source_pi (int_form 0))))
       then fail_out_of_running_or_sending_config (ConfigIdealSending c)
     else if eval_bool_form_to_bool c.gc pi dbs
